src/tls/concrete-flags/Flags.fst
@@ -2,15 +2,16 @@ module Flags
 
 // debug printing flags, one per module
 inline_for_extraction let debug = true
-inline_for_extraction let debug_HS = debug
-inline_for_extraction let debug_KS = debug
-inline_for_extraction let debug_TLS = debug
-inline_for_extraction let debug_NGO = debug
-inline_for_extraction let debug_HSL = debug
 inline_for_extraction let debug_CDH = debug
 inline_for_extraction let debug_Epochs = debug
 inline_for_extraction let debug_FFI = debug 
+inline_for_extraction let debug_HS = debug
+inline_for_extraction let debug_HSL = debug
+inline_for_extraction let debug_KS = debug
+inline_for_extraction let debug_NGO = debug
+inline_for_extraction let debug_QUIC = debug 
 inline_for_extraction let debug_Record = debug
+inline_for_extraction let debug_TLS = debug
 
 inline_for_extraction let ideal_KEF = false
 inline_for_extraction let ideal_Nonce = false  
