src/tls/HandshakeLog.fst
@@ -430,9 +430,9 @@ let rec parseMessages pvo kexo buf =
   | Error z -> Error z
   | Correct None -> trace "more bytes required"; Correct (false, buf, [], [])
   | Correct (Some (| rem, hstype, pl, to_log |)) ->
-    ( trace ("parsing " ^
-        (if pvo = Some TLS_1p3 then "(1.3) " else if pvo = Some TLS_1p2 then  "(1.2) " else "(?) ") ^
-        Platform.Bytes.print_bytes pl);
+    ( // trace ("parsing " ^
+      //   (if pvo = Some TLS_1p3 then "(1.3) " else if pvo = Some TLS_1p2 then  "(1.2) " else "(?) ") ^
+      //   Platform.Bytes.print_bytes pl);
       if hstype = HT_client_hello
       then (
         match parseClientHello pl with // ad hoc case: we parse into one or two messages
