src/tls/QUIC.fst
@@ -1,0 +1,101 @@
+module QUIC
+
+/// QUIC-specific interface on top of our main TLS API
+/// * establishes session & exported keys: no application-data traffic!
+/// * simplified configuration, with reasonable defaults
+/// * TCP-like send/recv callbacks operate on caller-provided buffers
+///   recv may yield (not enough input)
+///   send is guaranteed to succeed (large enough output buffer expected)
+///
+/// Relying on FFI for accessing configs, callbacks, etc.
+/// Testing both in OCaml (TCP-based, TestQUIC ~ TestFFI) and in C.
+
+open Platform.Bytes
+open Platform.Error
+open TLSConstants
+open TLSInfo
+open Range
+open DataStream
+open TLS
+open FFICallbacks
+
+open FStar.HyperStack.All
+
+#set-options "--lax"
+
+(* A flag for runtime debugging of ffi data.
+   The F* normalizer will erase debug prints at extraction
+   when this flag is set to false. *)
+val discard: bool -> ST unit
+  (requires (fun _ -> True))
+  (ensures (fun h0 _ h1 -> h0 == h1))
+let discard _ = ()
+let print s = discard (IO.debug_print_string ("QIC| "^s^"\n"))
+unfold val trace: s:string -> ST unit
+  (requires (fun _ -> True))
+  (ensures (fun h0 _ h1 -> h0 == h1))
+unfold let trace = if Flags.debug_QUIC then print else (fun _ -> ())
+
+
+// an integer carrying the fatal alert descriptor
+// we could also write txt into the application error log
+type error = bytes 
+private let errno description txt: ST error 
+  (requires fun h0 -> True)
+  (ensures fun h0 _ h1 -> h0 == h1) 
+=
+  trace ("returning error"^
+    (match description with
+    | Some ad -> " "^TLSError.string_of_ad ad
+    | None    -> "")^": "^txt);
+  Alert.alertBytes (match description with | Some a -> a | None -> TLSError.AD_internal_error)
+
+/// TLS processing loop: we keep receiving and sending as long as we
+/// can read.  Does not handle TLS termination (unused by QUIC?)
+/// 
+type result = 
+  | TLS_would_block // requires more input to continue
+  | TLS_error_local of error
+  | TLS_error_alert of error  
+  | TLS_secret0 // 0RTT exporter secret TODO
+  | TLS_secret1 // 1RTT exporter secret TODO
+  | TLS_ticket // server ticket TODO
+  | TLS_complete // signalling handshake completion
+  | TLS_refuse0 // TODO (still have to discard EOED)
+ // do we ever need to return multiple signals?
+
+val recv: Connection.connection -> St result
+let rec recv c = 
+  let i = currentId c Reader in 
+  match read c i with 
+  | Update false -> recv c // ignoring internal key changes
+  | ReadWouldBlock -> TLS_would_block
+  | Update true -> TLS_secret0 // TODO 0RTT, 0.5RTT, or 1RTT depending on c.
+  | Complete -> TLS_complete
+  | ReadError description txt -> TLS_error_local (errno description txt)
+  | Read Close -> TLS_error_alert (errno (Some TLSError.AD_close_notify) "received close")
+  | Read (Alert a) -> TLS_error_alert (errno (Some a) "received alert")
+  | _ -> TLS_error_local (errno None "unexpected TLS read result")
+
+/// Creation (no I/O yet)
+/// 
+let connect send recv client_config : ML Connection.connection =
+  // we assume the configuration specifies the target SNI;
+  // otherwise we should check after Complete that it matches the authenticated certificate chain.
+  let tcp = Transport.callbacks send recv in
+  let here = new_region HyperHeap.root in
+  TLS.connect here tcp client_config
+
+let accept send recv server_config : ML Connection.connection =
+  let tcp = Transport.callbacks send recv in
+  let here = new_region HyperHeap.root in
+  TLS.accept_connected here tcp server_config
+
+val ffiConnect: config:config -> callbacks:FFI.callbacks -> ML Connection.connection
+let ffiConnect config cb =
+  connect (FFI.sendTcpPacket cb) (FFI.recvTcpPacket cb) config
+
+val ffiAcceptConnected: config:config -> callbacks:FFI.callbacks -> ML Connection.connection
+let ffiAcceptConnected config cb =
+  accept (FFI.sendTcpPacket cb) (FFI.recvTcpPacket cb) config
+
