src/tls/ideal-flags/Flags.fst
@@ -2,15 +2,16 @@ module Flags
 
 // debug printing flags, one per module
 assume val debug : bool
-assume val debug_HS : bool
-assume val debug_KS : bool
-assume val debug_TLS : bool
-assume val debug_NGO : bool
-assume val debug_HSL : bool
 assume val debug_CDH : bool
 assume val debug_Epochs : bool
 assume val debug_FFI : bool
+assume val debug_HS : bool
+assume val debug_HSL : bool
+assume val debug_KS : bool
+assume val debug_NGO : bool
+assume val debug_QUIC : bool 
 assume val debug_Record : bool 
+assume val debug_TLS : bool
 
 assume val ideal_KEF : bool
 assume val ideal_Nonce : bool 
