src/tls/test/TestQUIC.fst
@@ -1,0 +1,72 @@
+module TestQUIC
+
+// a variant of TestAPI for testing QUIC.fst
+
+open FStar.Seq
+open FStar.HyperHeap
+open Platform.Bytes
+open Platform.Error
+open TLSError
+open TLSInfo
+open TLSConstants
+
+open FStar.HyperStack.All
+open FStar.HyperStack.ST
+
+open QUIC
+
+(* A flag for runtime debugging of Handshake data.
+   The F* normalizer will erase debug prints at extraction
+   when this flag is set to false. *)
+
+val discard: bool -> ST unit
+  (requires (fun _ -> True))
+  (ensures (fun h0 _ h1 -> h0 == h1))
+let discard _ = ()
+let print s = discard (IO.debug_print_string ("QIC| "^s^"\n"))
+let print_tcp s = discard (IO.debug_print_string ("TCP| "^s^"\n"))
+unfold val trace: s:string -> ST unit
+  (requires (fun _ -> True))
+  (ensures (fun h0 _ h1 -> h0 == h1))
+unfold let trace = if Flags.debug_QUIC then print else (fun _ -> ())
+unfold val trace_tcp: s:string -> ST unit
+  (requires (fun _ -> True))
+  (ensures (fun h0 _ h1 -> h0 == h1))
+unfold let trace_tcp = if Flags.debug_QUIC then print_tcp else (fun _ -> ())
+
+
+private let rec read c : ML QUIC.result = // auxiliary while loop for reading the full response
+  match recv c with
+  | TLS_would_block -> trace "blocked"; recv c
+  | TLS_secret0 -> trace "secret0"; recv c
+  | TLS_secret1 -> trace "secret1"; recv c
+  | TLS_ticket -> trace "ticket"; recv c
+//| TLS_complete -> trace "complete"
+  | r -> r
+
+let client config host port =
+  trace "CLIENT"; 
+  let tcp = Platform.Tcp.connect host port in 
+  let request = "GET / HTTP/1.1\r\nHost: " ^ host ^ "\r\n\r\n" in 
+  let send x = trace_tcp "send"; Platform.Tcp.send tcp x in
+  let recv x = trace_tcp "recv"; Platform.Tcp.recv_async tcp x in
+  let c = QUIC.connect send recv config in
+  let _ = read c in 
+  trace "OK\n"
+
+let single_server config client : ML unit =
+  let send x = trace_tcp "send"; Platform.Tcp.send client x in
+  let recv x = trace_tcp "recv"; Platform.Tcp.recv_async client x in
+  let c = QUIC.accept send recv config in
+  let _ = read c in
+  trace "OK\n"
+ 
+let rec aux_server config sock : ML unit =
+ let client = Platform.Tcp.accept sock in
+ let _ = single_server config client in
+ aux_server config sock
+
+let server config host port =
+ trace "SERVER";
+ let sock = Platform.Tcp.listen host port in
+ aux_server config sock
